tests/core.v
@@ -6,3 +6,19 @@ Redirect "core1.log" Lean Import "../dumps/core" 1 5584.
 Fail Redirect "core2.log" Lean Import "../dumps/core" 5584 63566.
 
 (* Redirect "core3.log" Lean Import "../dumps/core" 5086 63566. *)
+
+Set Printing Universes.
+Print String.
+Print Char.
+Print UInt32.
+Eval hnf in LT_lt_inst1 Nat instLTNat.
+Print Nat_le.
+Print Or.
+Print And.
+Print Fin.
+Print UInt32_isValidChar.
+Print Nat_isValidChar.
+Print UInt32_toNat.
+(* Compute Z.of_nat (nat_of_Nat UInt32_size. *)
+(* n < 0xd800 ∨ (0xdfff < n ∧ n < 0x110000) *)
+(* Eval hnf in UInt32_isValidChar _. *)
